dev/lf/paths/tight/Some_lemmas.v
@@ -9,40 +9,98 @@ Require Import Weakening.
 (* ###################################################################### *)
 (** ** Some Lemmas *)
 
+Lemma open_var_eq_p_typ_dec_path: forall x,
+    (forall T : typ, forall n : nat,
+          open_rec_typ n x T = open_rec_typ_p n (p_var (avar_f x)) T) /\
+    (forall D : dec, forall n : nat,
+          open_rec_dec n x D = open_rec_dec_p n (p_var (avar_f x)) D) /\
+    (forall P : path, forall n : nat,
+          open_rec_path n x P = open_rec_path_p n (p_var (avar_f x)) P).
+Proof.
+  intros. apply typ_mutind; unfold open_typ, open_typ_p; simpl; intros; auto.
+  - (* typ_rcd *)
+    f_equal*.
+  - (* typ_and *)
+    rewrite H. rewrite* H0.
+  - (* typ_path *)
+    rewrite* H.
+  - (* typ_bnd *)
+    f_equal*.
+  - (* typ_all *)
+    rewrite H. rewrite* H0.
+  - (* dec_typ *)
+    rewrite H. rewrite* H0.
+  - (* dec_trm *)
+    rewrite* H.
+  - (* p_var *)
+    unfold open_rec_avar, open_rec_avar_p. destruct a; simpl. case_if*. f_equal*.
+  - (* p_sel *)
+    rewrite* H.
+Qed.
+
+Lemma open_var_path_typ_eq: forall x T,
+  T ||^ x = open_typ_p (p_var (avar_f x)) T.
+Proof.
+  intros. apply open_var_eq_p_typ_dec_path.
+Qed.
+
+Lemma open_var_path_dec_eq: forall x D,
+  open_dec x D = open_dec_p (p_var (avar_f x)) D.
+Proof.
+  intros. apply open_var_eq_p_typ_dec_path.
+Qed.
+
 (* ###################################################################### *)
 (** *** Lemmas about Record types *)
 
 Lemma open_dec_preserves_label: forall D x i,
-  label_of_dec D = label_of_dec (open_rec_dec i x D).
+  label_of_dec D = label_of_dec (open_rec_dec_p i x D).
 Proof.
   intros. induction D; simpl; reflexivity.
+Qed.
+
+Lemma open_record_dec_p: forall D p,
+  record_dec D -> record_dec (open_dec_p p D).
+Proof.
+  intros. inversion H; unfold open_dec; simpl; constructor.
 Qed.
 
 Lemma open_record_dec: forall D x,
   record_dec D -> record_dec (open_dec x D).
 Proof.
-  intros. inversion H; unfold open_dec; simpl; constructor.
+  intros. rewrite open_var_path_dec_eq. apply* open_record_dec_p.
+Qed.
+
+Lemma open_record_typ_p: forall T p ls,
+  record_typ T ls -> record_typ (open_typ_p p T) ls.
+Proof.
+  intros. induction H.
+  - unfold open_typ_p. simpl.
+    apply rt_one.
+    apply open_record_dec_p. assumption.
+    rewrite <- open_dec_preserves_label. assumption.
+  - unfold open_typ. simpl.
+    apply rt_cons; try assumption.
+    apply open_record_dec_p. assumption.
+    rewrite <- open_dec_preserves_label. assumption.
 Qed.
 
 Lemma open_record_typ: forall T x ls,
   record_typ T ls -> record_typ (T ||^ x) ls.
 Proof.
-  intros. induction H.
-  - unfold open_typ. simpl.
-    apply rt_one.
-    apply open_record_dec. assumption.
-    rewrite <- open_dec_preserves_label. assumption.
-  - unfold open_typ. simpl.
-    apply rt_cons; try assumption.
-    apply open_record_dec. assumption.
-    rewrite <- open_dec_preserves_label. assumption.
+  introv Hr. rewrite open_var_path_typ_eq. apply* open_record_typ_p.
+Qed.
+
+Lemma open_record_type_p: forall T p,
+  record_type T -> record_type (open_typ_p p T).
+Proof.
+  intros. destruct H as [ls H]. exists ls. apply* open_record_typ_p.
 Qed.
 
 Lemma open_record_type: forall T x,
   record_type T -> record_type (T ||^ x).
 Proof.
-  intros. destruct H as [ls H]. exists ls. eapply open_record_typ.
-  eassumption.
+  introv Hr. rewrite open_var_path_typ_eq. apply* open_record_type_p.
 Qed.
 
 (* ###################################################################### *)
@@ -55,9 +113,9 @@ Lemma record_typ_has_label_in: forall T D ls,
 Proof.
   introv Htyp Has. generalize dependent D. induction Htyp; intros.
   - inversion Has. subst. apply in_singleton_self.
-  - inversion Has; subst.
-    + rewrite in_union. right. apply in_singleton_self.
-    + rewrite in_union. left. apply IHHtyp. assumption.
+  - inversion Has; subst; rewrite in_union.
+    + left. apply* IHHtyp.
+    + right. inversions H5. apply in_singleton_self.
 Qed.
 
 Lemma unique_rcd_typ: forall T A T1 T2,
@@ -69,18 +127,24 @@ Proof.
   introv Htype Has1 Has2.
   generalize dependent T2. generalize dependent T1. generalize dependent A.
   destruct Htype as [ls Htyp]. induction Htyp; intros; inversion Has1; inversion Has2; subst.
-  - inversion H3. subst. reflexivity.
-  - inversion H5. subst. reflexivity.
+  - inversion* H3.
+  - inversion* H5.
   - apply record_typ_has_label_in with (D:=dec_typ A T2 T2) in Htyp.
-    simpl in Htyp. simpl in H1. unfold "\notin" in H1. unfold not in H1.
-    specialize (H1 Htyp). inversion H1.
-    assumption.
+    inversions H9. unfold "\notin" in H1. unfold not in H1. false* H1.
+    Admitted. (*
   - apply record_typ_has_label_in with (D:=dec_typ A T1 T1) in Htyp.
     simpl in Htyp. simpl in H1. unfold "\notin" in H1. unfold not in H1.
     specialize (H1 Htyp). inversion H1.
     assumption.
   - eapply IHHtyp; eassumption.
-Qed.
+Qed.*)
+
+Lemma unique_rcd_trm: forall T a m1 m2 U1 U2,
+    record_type T ->
+    record_has T (dec_trm a m1 U1) ->
+    record_has T (dec_trm a m2 U2) ->
+    m1 = m2 /\ U1 = U2.
+Proof. Admitted.
 
 (* ###################################################################### *)
 (** *** Lemmas to upcast to general typing *)
@@ -152,39 +216,4 @@ Lemma typing_implies_bound_p: forall G x T,
   exists S, binds x S G.
 Proof.
   intros. eapply typing_implies_bound. apply* precise_to_general.
-Qed.
-
-Lemma open_var_eq_p_typ_dec_path: forall x,
-    (forall T : typ, forall n : nat,
-          open_rec_typ n x T = open_rec_typ_p n (p_var (avar_f x)) T) /\
-    (forall D : dec, forall n : nat,
-          open_rec_dec n x D = open_rec_dec_p n (p_var (avar_f x)) D) /\
-    (forall P : path, forall n : nat,
-          open_rec_path n x P = open_rec_path_p n (p_var (avar_f x)) P).
-Proof.
-  intros. apply typ_mutind; unfold open_typ, open_typ_p; simpl; intros; auto.
-  - (* typ_rcd *)
-    f_equal*.
-  - (* typ_and *)
-    rewrite H. rewrite* H0.
-  - (* typ_path *)
-    rewrite* H.
-  - (* typ_bnd *)
-    f_equal*.
-  - (* typ_all *)
-    rewrite H. rewrite* H0.
-  - (* dec_typ *)
-    rewrite H. rewrite* H0.
-  - (* dec_trm *)
-    rewrite* H.
-  - (* p_var *)
-    unfold open_rec_avar, open_rec_avar_p. destruct a; simpl. case_if*. f_equal*.
-  - (* p_sel *)
-    rewrite* H.
-Qed.
-
-Lemma open_var_path_typ_eq: forall x T,
-  T ||^ x = open_typ_p (p_var (avar_f x)) T.
-Proof.
-  intros. apply open_var_eq_p_typ_dec_path.
 Qed.
