dev/lf/paths/tight/Tight_possible_types.v
@@ -3,7 +3,6 @@ Set Implicit Arguments.
 Require Import LibLN.
 Require Import Coq.Program.Equality.
 Require Import Definitions.
-Require Import Precise_flow.
 Require Import Inert_types.
 
 (* ###################################################################### *)
@@ -28,14 +27,18 @@ Reserved Notation "G '|-##' p '::' T" (at level 40, p at level 59).
 
 Inductive tight_pt : ctx -> path -> typ -> Prop :=
   (* Precise typing *)
-| t_pt_precise : forall G x T,
-    G |-! trm_path (p_var (avar_f x)) :: T ->
-    G |-## p_var (avar_f x) :: T
-  (* Term member subtyping *)
-| t_pt_dec_trm : forall G p a m T T',
-    G |-## p :: typ_rcd (dec_trm a m T) ->
+| t_pt_precise : forall G p T,
+    G |-! trm_path p :: T ->
+    G |-## p :: T
+  (* General term member subtyping *)
+| t_pt_dec_trm : forall G p a T T',
+    G |-## p :: typ_rcd (dec_trm a general T) ->
     G |-# T <: T' ->
-    G |-## p :: typ_rcd (dec_trm a m T')
+    G |-## p :: typ_rcd (dec_trm a general T')
+  (* Strong term member subtyping *)
+| t_pt_dec_trm_strong : forall G p a T,
+    G |-## p :: typ_rcd (dec_trm a strong T) ->
+    G |-## p :: typ_rcd (dec_trm a general T)
   (* Type member subtyping *)
 | t_pt_dec_typ : forall G p A T T' U' U,
     G |-## p :: typ_rcd (dec_typ A T U) ->
@@ -43,9 +46,9 @@ Inductive tight_pt : ctx -> path -> typ -> Prop :=
     G |-# U <: U' ->
     G |-## p :: typ_rcd (dec_typ A T' U')
   (* Recursive Types *)
-| t_pt_bnd : forall G p S,
-    G |-## p :: open_typ_p p S ->
-    G |-## p :: typ_bnd S
+| t_pt_bnd : forall G x S,
+    G |-## (p_var (avar_f x)) :: S ||^ x ->
+    G |-## (p_var (avar_f x)) :: typ_bnd S
   (* Forall *)
 | t_pt_all : forall L G p S T S' T',
     G |-## p :: typ_all S T ->
@@ -54,14 +57,15 @@ Inductive tight_pt : ctx -> path -> typ -> Prop :=
       G & y ~ S' |- T ||^ y <: T' ||^ y) ->
     G |-## p :: typ_all S' T'
   (* And *)
-| t_pt_and : forall G p S1 S2,
-    G |-## p :: S1 ->
-    G |-## p :: S2 ->
-    G |-## p :: typ_and S1 S2
+| t_pt_and : forall G p S T,
+    G |-## p :: S ->
+    G |-## p :: T ->
+    G |-## p :: typ_and S T
   (* Tight Selection *)
 | t_pt_sel : forall G p q A S,
     G |-## p :: S ->
     G |-! trm_path q :: typ_rcd (dec_typ A S S) ->
+    norm_t G q ->
     G |-## p :: typ_path q A
   (* Top *)
 | t_pt_top : forall G p T,
@@ -77,27 +81,27 @@ Lemma tight_possible_types_closure_tight: forall G p T U,
   G |-# T <: U ->
   G |-## p :: U.
 Proof.
-  introv Hgd HT Hsub.
+  introv Hi HT Hsub.
   dependent induction Hsub; eauto.
-  - inversion HT. inversions H1.
-    destruct (inert_ty_precise_bot Hgd H).
+  - inversions HT. false* precise_bot_false.
   - inversion* HT.
   - inversion* HT.
   - inversions HT.
-    + false * inert_precise_sel_inv.
-    + pose proof (inert_unique_tight_bounds Hgd H H5) as Hu. subst. assumption.
+    + false *precise_psel_false.
+    + pose proof (inert_unique_tight_bounds Hi H H6). subst. assumption.
 Qed.
 
-Lemma tight_possible_types_lemma :
-  forall G U x,
+Lemma tight_possible_types_lemma : forall G U p,
     inert G ->
-    G |-# trm_var (avar_f x) :: U ->
-    G |-## x :: U.
+    G |-# trm_path p :: U ->
+    G |-## p :: U.
 Proof.
-  intros G U x Hgd Hty.
-  dependent induction Hty.
-  - auto.
-  - specialize (IHHty _ Hgd eq_refl eq_refl eq_refl).
+  introv Hi Hty.
+  dependent induction Hty; auto.
+  - specialize (IHHty p0  Hi eq_refl). inversions IHHty.
+    * apply ty_fld_elim_p in H. auto.
+
+    specialize (IHHty _ Hgd eq_refl eq_refl eq_refl).
     eapply t_pt_bnd.
     apply IHHty.
     reflexivity.
